Clean Core.Blake2 + Add better placeholders for hash and update_multi for Blake2

code/hash/Hacl.Hash.Blake2.fst
@@ -1,16 +1,53 @@
 module Hacl.Hash.Blake2
 
+module B = LowStar.Buffer
+module ST = FStar.HyperStack.ST
+module M = LowStar.Modifies
+
+open Lib.IntTypes
+
+module Spec = Spec.Blake2
+module Impl = Hacl.Impl.Blake2.Generic
+module Core = Hacl.Impl.Blake2.Core
+
+open FStar.Mul
+
+#set-options "--fuel 0 --ifuel 0"
+
+#push-options "--fuel 1 --ifuel 1"
+
+noextract inline_for_extraction
+val mk_update_multi: a:hash_alg{is_blake a} -> update:update_st a -> update_multi_st a
+
+let mk_update_multi a update s ev block n_blocks =
+  let h0 = ST.get () in
+  admit()
+
+#pop-options
+
 let update_multi_blake2s: update_multi_st Blake2S =
-  admit()
+  mk_update_multi Blake2S update_blake2s
 let update_multi_blake2b: update_multi_st Blake2B =
-  admit()
+  mk_update_multi Blake2B update_blake2b
 
 let update_last_blake2s: update_last_st Blake2S =
   admit()
 let update_last_blake2b: update_last_st Blake2B =
   admit()
 
-let hash_blake2s: hash_st Blake2S =
-  admit()
-let hash_blake2b: hash_st Blake2B =
-  admit()
+let lemma_blake2_hash_equivalence
+  (a:hash_alg{is_blake a}) (d:bytes{Seq.length d <= max_input_length a})
+  : Lemma
+    (Spec.blake2 (to_blake_alg a) d 0 Seq.empty (Spec.max_output (to_blake_alg a)) ==
+     Spec.Agile.Hash.hash a d)
+  = admit()
+
+let hash_blake2s: hash_st Blake2S = fun input input_len dst ->
+  let h0 = ST.get() in
+  Hacl.Blake2s_32.blake2s 32ul dst input_len input 0ul (B.null #uint8);
+  lemma_blake2_hash_equivalence Blake2S (B.as_seq h0 input)
+
+let hash_blake2b: hash_st Blake2B = fun input input_len dst ->
+  let h0 = ST.get() in
+  Hacl.Blake2b_32.blake2b 64ul dst input_len input 0ul (B.null #uint8);
+  lemma_blake2_hash_equivalence Blake2B (B.as_seq h0 input)
